src/typechecker/FStar.TypeChecker.NBETerm.fsti
@@ -37,6 +37,8 @@ module Z = FStar.BigInt
 module C = FStar.Const
 open FStar.Char
 
+val interleave_hack : int
+
 (*
    This module provides the internal term representations used in the
    NBE algorithm implemented by FStar.TypeChecker.NBE.fs (see the
@@ -200,6 +202,15 @@ and cflag =
 and arg = t * aqual
 and args = list (arg)
 
+val isAccu : t -> bool
+val isNotAccu : t -> bool
+
+val mkConstruct : fv -> list universe -> args -> t
+val mkFV : fv -> list universe -> args -> t
+
+val mkAccuVar : var -> t
+val mkAccuMatch : t -> (unit -> option match_returns_ascription) -> (unit -> list branch) -> (unit -> option S.residual_comp) -> t
+
 type head = t
 type annot = option t
 
@@ -208,11 +219,12 @@ type nbe_cbs = {
    translate : term -> t;
 }
 
-type embedding 'a = {
-  em  : nbe_cbs -> 'a -> t;
-  un  : nbe_cbs -> t -> option 'a;
-  typ : t;
-  emb_typ : emb_typ
+type embedding (a:Type0) = {
+  em  : nbe_cbs -> a -> t;
+  un  : nbe_cbs -> t -> option a;
+  (* thunking to allow total instances *)
+  typ : unit -> t;
+  emb_typ : unit -> emb_typ;
 }
 
 // Printing functions
@@ -226,14 +238,6 @@ val args_to_string : args -> string
 // NBE term manipulation
 val mk_t : t' -> t
 val nbe_t_of_t : t -> t'
-val isAccu : t -> bool
-val isNotAccu : t -> bool
-
-val mkConstruct : fv -> list universe -> args -> t
-val mkFV : fv -> list universe -> args -> t
-
-val mkAccuVar : var -> t
-val mkAccuMatch : t -> (unit -> option match_returns_ascription) -> (unit -> list branch) -> (unit -> option S.residual_comp) -> t
 
 val as_arg : t -> arg
 val as_iarg : t -> arg
@@ -243,9 +247,9 @@ val translate_cb : nbe_cbs -> term -> t
 
 val mk_emb : (nbe_cbs -> 'a -> t) ->
              (nbe_cbs -> t -> option 'a) ->
-             t ->
-             emb_typ ->
-             embedding 'a
+             (unit -> t) ->
+             (unit -> emb_typ) ->
+             Prims.Tot (embedding 'a)
 
 val embed_as : embedding 'a -> ('a -> 'b) -> ('b -> 'a) -> option t -> embedding 'b
 
@@ -267,11 +271,11 @@ val e_issue  : embedding FStar.Errors.issue
 val e_document : embedding FStar.Pprint.document
 val e_vconfig  : embedding vconfig
 val e_norm_step : embedding Pervasives.norm_step
-val e_list   : embedding 'a -> embedding (list 'a)
-val e_option : embedding 'a -> embedding (option 'a)
-val e_tuple2 : embedding 'a -> embedding 'b -> embedding ('a * 'b)
-val e_tuple3 : embedding 'a -> embedding 'b -> embedding 'c -> embedding ('a * 'b * 'c)
-val e_either : embedding 'a -> embedding 'b -> embedding (either 'a 'b)
+val e_list   : #a:Type -> embedding a -> Prims.Tot (embedding (list a))
+val e_option : embedding 'a -> Prims.Tot (embedding (option 'a))
+val e_tuple2 : embedding 'a -> embedding 'b -> Prims.Tot (embedding ('a * 'b))
+val e_tuple3 : embedding 'a -> embedding 'b -> embedding 'c -> Prims.Tot (embedding ('a * 'b * 'c))
+val e_either : embedding 'a -> embedding 'b -> Prims.Tot (embedding (either 'a 'b))
 val e_sealed : embedding 'a -> embedding 'a
 val e_string_list : embedding (list string)
 val e_arrow : embedding 'a -> embedding 'b -> embedding ('a -> 'b)
