src/tactics/FStar.Tactics.V1.Interpreter.fst
@@ -60,8 +60,9 @@ module PO      = FStar.TypeChecker.Primops
 
 let tacdbg = BU.mk_ref false
 
-let unembed ea a norm_cb = unembed ea a norm_cb
-let embed ea r x norm_cb = embed ea x r None norm_cb
+(* No typeclasses in this module, it's deprecated anyway *)
+let unembed ea a norm_cb = unembed #_ #ea a norm_cb
+let embed ea r x norm_cb = embed #_ #ea x r None norm_cb
 
 let native_tactics_steps () =
   let step_from_native_step (s: native_primitive_step): PO.primitive_step =
@@ -227,8 +228,8 @@ let e_tactic_nbe_thunk (er : NBET.embedding 'r) : NBET.embedding (tac 'r)
     NBET.mk_emb
            (fun cb _ -> failwith "Impossible: NBE embedding tactic (thunk)?")
            (fun cb t -> Some (unembed_tactic_nbe_1 NBET.e_unit er cb t ()))
-           (NBET.mk_t (NBET.Constant NBET.Unit))
-           (emb_typ_of e_unit)
+           (fun () -> NBET.mk_t (NBET.Constant NBET.Unit))
+           (emb_typ_of unit)
 
 let e_tactic_1 (ea : embedding 'a) (er : embedding 'r) : embedding ('a -> tac 'r)
     =
@@ -241,8 +242,8 @@ let e_tactic_nbe_1 (ea : NBET.embedding 'a) (er : NBET.embedding 'r) : NBET.embe
     NBET.mk_emb
            (fun cb _ -> failwith "Impossible: NBE embedding tactic (1)?")
            (fun cb t -> Some (unembed_tactic_nbe_1 ea er cb t))
-           (NBET.mk_t (NBET.Constant NBET.Unit))
-           (emb_typ_of e_unit)
+           (fun () -> NBET.mk_t (NBET.Constant NBET.Unit))
+           (emb_typ_of unit)
 
 (* Set the primitive steps ref *)
 let () =
