src/tactics/FStar.Tactics.V2.InterpFuns.fst
@@ -40,8 +40,9 @@ module NBETerm = FStar.TypeChecker.NBETerm
 module NBET    = FStar.TypeChecker.NBETerm
 module PO    = FStar.TypeChecker.Primops
 
-let unembed e t n = FStar.Syntax.Embeddings.unembed e t n
-let embed e rng t n = FStar.Syntax.Embeddings.embed e t rng None n
+(* This module does not use typeclasses *)
+let embed (e:embedding 'a) rng (t:'a) n = FStar.Syntax.Embeddings.embed #_ #e t rng None n
+let unembed (e:embedding 'a) t n : option 'a = FStar.Syntax.Embeddings.unembed #_ #e t n
 
 let rec drop n l =
     if n = 0 then l
