src/typechecker/FStar.TypeChecker.Normalize.fst
@@ -624,7 +624,7 @@ let closure_as_term cfg env t = non_tail_inline_closure_env cfg env t
 let unembed_binder_knot : ref (option (EMB.embedding binder)) = BU.mk_ref None
 let unembed_binder (t : term) : option S.binder =
     match !unembed_binder_knot with
-    | Some e -> EMB.try_unembed e t EMB.id_norm_cb
+    | Some e -> EMB.try_unembed #_ #e t EMB.id_norm_cb
     | None ->
         Errors.log_issue t.pos (Errors.Warning_UnembedBinderKnot, "unembed_binder_knot is unset!");
         None
@@ -723,7 +723,7 @@ let reduce_primops norm_cb cfg env tm : term & bool =
            log_primops cfg (fun () -> BU.print1 "primop: reducing <%s>\n"
                                         (Print.term_to_string tm));
            begin match args with
-           | [(a1, _)] -> PO.embed_simple EMB.e_range a1.pos tm.pos, false
+           | [(a1, _)] -> PO.embed_simple a1.pos tm.pos, false
            | _ -> tm, false
            end
 
@@ -732,7 +732,7 @@ let reduce_primops norm_cb cfg env tm : term & bool =
                                         (Print.term_to_string tm));
            begin match args with
            | [(t, _); (r, _)] ->
-                begin match PO.try_unembed_simple EMB.e_range r with
+                begin match PO.try_unembed_simple r with
                 | Some rng -> Subst.set_use_range rng t, false
                 | None -> tm, false
                 end
@@ -793,7 +793,7 @@ let is_nbe_request s = BU.for_some (eq_step NBE) s
 
 let get_norm_request cfg (full_norm:term -> term) args =
     let parse_steps s =
-      match PO.try_unembed_simple (EMB.e_list EMB.e_norm_step) s with
+      match PO.try_unembed_simple s with
       | Some steps -> Some (Cfg.translate_norm_steps steps)
       | None -> None
     in
@@ -1952,16 +1952,16 @@ and do_reify_monadic fallback cfg env stack (top : term) (m : monad_name) (t : t
 
                   let range_args =
                     if bind_has_range_args
-                    then [as_arg (PO.embed_simple EMB.e_range lb.lbpos lb.lbpos);
-                          as_arg (PO.embed_simple EMB.e_range body.pos body.pos)]
+                    then [as_arg (PO.embed_simple lb.lbpos lb.lbpos);
+                          as_arg (PO.embed_simple body.pos body.pos)]
                     else [] in
 
                   (S.as_arg lb.lbtyp)::(S.as_arg t)::(unit_args@range_args@[S.as_arg f_arg; S.as_arg body])
                 else
                   let maybe_range_arg =
                     if BU.for_some (U.attr_eq U.dm4f_bind_range_attr) ed.eff_attrs
-                    then [as_arg (PO.embed_simple EMB.e_range lb.lbpos lb.lbpos);
-                          as_arg (PO.embed_simple EMB.e_range body.pos body.pos)]
+                    then [as_arg (PO.embed_simple lb.lbpos lb.lbpos);
+                          as_arg (PO.embed_simple body.pos body.pos)]
                     else []
                   in
                   [ (* a, b *)
